theories/sups.v
@@ -15,11 +15,11 @@ Lemma geq_is_sup P x: is_sup P x -> forall z, (forall y, P y -> y <= z) -> x <= 
 Proof. by move=>H z Hz; apply H. Qed.
 
 Lemma leq_is_sup P x: is_sup P x -> forall y, P y -> y <= x.
-Proof. by move=>H y Py; apply H. Qed.
+Proof. move=>H y Py. by apply H. Qed.
 
 Lemma is_sup_leq P p Q q: is_sup P p -> is_sup Q q -> covered P Q -> p<=q.
 Proof.
-  move=>Pp Qq PQ. apply Pp=>x Px.
+  move=>Pp Qq PQ. apply Pp=>x Px/=.
   case: (PQ x Px)=>y [Qy ->]. by apply Qq.
 Qed.
 
@@ -29,10 +29,10 @@ Proof. rewrite eqv_of_leq=>??[??]. eauto using is_sup_leq. Qed.
 Lemma is_sup_unique (P: X -> Prop) x y: is_sup P x -> is_sup P y -> x ≡ y.
 Proof. intros; eapply is_sup_eqv; eauto. Qed.
 
-Lemma is_sup_single x: is_sup (eq x) x.
-Proof. intro. by firstorder subst. Qed.
+Lemma is_sup_eq x: is_sup (eq x) x.
+Proof. move=>/=. rewrite /upper_bound. by firstorder subst. Qed.
 
-#[export] Instance Proper_is_sup: Proper (bicovered ==> eqv ==> eqv) (@is_sup X).
+#[export] Instance Proper_is_sup: Proper (bicovered ==> eqv ==> iff) (@is_sup X).
 Proof.
   rewrite /is_sup=> P Q PQ x y xy.
   apply Proper_forall=>z. apply Proper_iff. by rewrite xy.
@@ -44,7 +44,7 @@ Qed.
 Lemma sup_closed_impl (P Q: X -> Prop): Proper (leq --> leq) P -> sup_closed Q -> sup_closed (fun x => P x -> Q x).
 Proof.
   intros HP HQ T TPQ x Tx Px.
-  eapply HQ. 2: apply Tx.
+  apply: HQ. 2: apply Tx.
   intros y Ty. apply: TPQ=>//.
   apply: HP. 2: apply Px.
   by apply Tx. 
@@ -61,7 +61,7 @@ Lemma sup_closed_Proper P: sup_closed P -> Proper (eqv ==> eqv) P.
 Proof.
   move=>H. apply/Proper_eqv_leq. 
   move=>x y xy Px. apply: (H (eq x)). by move=>?<-. 
-  move: (is_sup_single x). by apply Proper_is_sup. 
+  move: (is_sup_eq x). by apply Proper_is_sup. 
 Qed.
 
 Inductive sup_closure P: X -> Prop :=
@@ -78,23 +78,37 @@ Proof.
   - elim: Px=>//Q QP IH y Hy. apply Hy. exact: IH.
 Qed.
 
-Lemma is_sup_empty z:
-  is_sup empty z <-> forall t, z <= t.
-Proof. rewrite /is_sup. setoid_rewrite forall_empty. firstorder. Qed.
+
+#[export] Instance sup_closure_set P: Proper (eqv ==> eqv) (sup_closure P).
+Proof. apply: sup_closed_Proper. exact/sc_sup. Qed.
+HB.instance Definition _ P := isExtensional.Build _ _ (sup_closure P) (sup_closure_set P).
+
+Lemma is_sup_empty z: is_sup empty z <-> forall t, z <= t.
+Proof.
+  rewrite /is_sup. setoid_rewrite upper_bound_empty.
+  firstorder.
+Qed.
+
+Lemma is_sup_single x y: is_sup (single x) y ≡ (x ≡ y).
+Proof.
+  rewrite /is_sup. setoid_rewrite upper_bound_single.
+  split. symmetry. exact/from_above.
+  move=>e?. by rewrite e.
+Qed.
 
 Lemma is_sup_pair x y z:
   is_sup (pair x y) z <-> forall t, z <= t <-> x <= t /\ y <= t.
-Proof. rewrite /is_sup. by setoid_rewrite forall_pair. Qed.
+Proof. rewrite /is_sup. by setoid_rewrite upper_bound_pair. Qed.
 
 Lemma is_sup_image {A} (f: A -> X) (P: A -> Prop) z:
   is_sup (image f P) z <-> forall t, z <= t <-> forall a, P a -> f a <= t.
-Proof. rewrite /is_sup. by setoid_rewrite forall_image. Qed.
+Proof. rewrite /is_sup. by setoid_rewrite upper_bound_image. Qed.
 
 End s.
 
 (** sups can be computed pointwise in function spaces *)
 Lemma dprod_sup {A} {X: A -> PO.type} (P: (forall a, X a) -> Prop) (f: forall a, X a):
-  (forall a, is_sup (image (app a) P) (f a)) -> is_sup P f.
+  (forall a: A, is_sup (image (app a) P) (f a)) -> is_sup P f.
 Proof.
   move=>H g; split=>fg.
   - move=>h Ph. rewrite -fg=>a. apply H=>//. by exists h.
@@ -103,8 +117,8 @@ Qed.
 (** sups being unique, they *must* be computed pointwise if they can
     (i.e., when there are enough sups in X) *)
 Lemma dprod_sup' {A} {X: A -> PO.type} (P: (forall a, X a) -> Prop) (f g: forall a, X a):
-  (forall a, is_sup (image (app a) P) (f a)) -> 
-  is_sup P g -> forall a, is_sup (image (app a) P) (g a).
+  (forall a: A, is_sup (image (app a) P) (f a)) -> 
+  is_sup P g -> forall a: A, is_sup (image (app a) P) (g a).
 Proof.
   move=>Pf Pg.
   have Pf': is_sup P f by apply: dprod_sup.
@@ -115,9 +129,9 @@ Qed.
 Lemma dprod_sup'' {A} {X: A -> PO.type}
       (A_dec: forall a b: A, {a=b} + {a<>b})
       (P: (forall a, X a) -> Prop) (f: forall a, X a):
-  is_sup P f -> forall a, is_sup (image (app a) P) (f a).
+  is_sup P f -> forall a: A, is_sup (image (app a) P) (f a).
 Proof.
-  move=>Pf a. split=>az.
+  move=>Pf a z. split=>az.
   - move=>_ [b [Pb ->]]. rewrite -az. by apply: (leq_is_sup Pf).
   - set h := fun b =>
                match A_dec a b return X b with
@@ -164,7 +178,7 @@ Lemma kern_sup {A} {X: PO.type} (f: A -> X) (P: kernel f->Prop) (a: kernel f):
   is_sup (image f P) (f a) -> is_sup P a.
 Proof.
   move=>H b; split=>ab.
-  -- move=>c Pc. rewrite -ab. by apply H; auto. 
+  -- move=>c Pc. rewrite -ab. by apply H, in_image. 
   -- apply H=>_ [c [Pc ->]]. by apply ab.
 Qed.
 
@@ -217,20 +231,24 @@ HB.end.
 (** sups on sub-spaces *)
 Section sub.
  Context {k} {X: gsupPO.type k}.
- Definition gsup_closed (P: X -> Prop) := forall I Q (kIQ: k I Q) (h: I -mon-> X), image h Q <= P -> P (gsup I Q kIQ h). 
+ (* TOTHINK: restrict to [P: set X] ? *)
+ Definition gsup_closed (P: X -> Prop) := forall I Q (kIQ: k I Q) (h: I -mon-> X), Q <= P ∘ h -> P (gsup I Q kIQ h). 
  Lemma sup_gsup_closed: sup_closed <= gsup_closed. 
- Proof. move=>P HP I Q kIQ h hQP. apply: HP. exact: hQP. exact: gsup_spec. Qed.
+ Proof.
+   move=>P HP. move: (sup_closed_Proper HP)=>HP' I Q kIQ h hQP.
+   apply: HP. 2: exact: gsup_spec. by apply (image_adj h _ (mk_set HP')).
+ Qed.
  #[export] Instance gsup_closed_eqv: Proper (eqv==>eqv) gsup_closed.
  Proof.
    apply/Proper_eqv_leq=>P P' PP' HP I Q kIQ h hQP'.
-   apply/PP'. apply: HP. by rewrite hQP' PP'.
- Qed.
+   apply/PP'. apply: HP. rewrite hQP'. apply: eqv_geq=>i. exact/PP'.
+ Qed. 
  
  Definition sup_closed_sig P (HP: gsup_closed P) := sig P.
  Variables (P: X -> Prop) (HP: gsup_closed P). 
  Program Definition sig_gsup I Q (kIQ: k I Q) (h: I -mon-> sig P): sig P :=
    exist P (gsup I Q kIQ (sval ∘ h)) _.
- Next Obligation. apply: HP. apply/forall_image=>i Qi. exact: proj2_sig. Qed.
+ Next Obligation. apply: HP=>i Qi/=. exact: proj2_sig. Qed.
  Lemma sig_gsup_spec I Q kIQ (h: I -mon-> sig P):
    is_sup (image h Q) (@sig_gsup I Q kIQ h).
  Proof. apply: kern_sup=>/=. rewrite -image_comp. exact: gsup_spec. Qed.
@@ -249,16 +267,16 @@ Section s.
    apply: (pointwise_sup_mon (F:=image h Q ∘ pobody))=>x. 
    eapply Proper_is_sup. 2: reflexivity. 2: exact: gsup_spec.
    split.
-   - move=>? [g [[i [Qi E]] ->]]. eexists; split. exists i; split=>//. by rewrite /app/= E.
+   - move=>? [g [[i [Qi E]] ->]]. eexists; split. exists i; split=>//. by rewrite /app/= (E x).
    - move=>? [i [Qi ->]].
-     have E: Proper (leq ==> leq) (h i) by apply: hQ; exact: in_image.
+     have E: Proper (leq ==> leq) (h i) by apply: hQ. 
      eexists; split. exists (mk_mon _ E); split=>//. exists i; split=>//. reflexivity.
    (* direct proof *)
    Restart.
    move=>I Q kIQ h hQ x y xy.
    rewrite gsup_spec=>z [i [Qi ->]].
    transitivity (h i y).
-   have E: Proper (leq ==> leq) (h i) by apply: hQ; exact: in_image.
+     have E: Proper (leq ==> leq) (h i) by apply: hQ. 
    by rewrite -xy.
    apply: leq_is_sup. apply gsup_spec. exact: in_image. 
  Qed.
@@ -285,9 +303,9 @@ Lemma adj_gsup {k} {X Y: gsupPO.type k} (f: X ⊣ Y) I P kIP h:
   f (@gsup k X I P kIP h) ≡ gsup I P kIP (f ∘ h). 
 Proof.
   apply: from_above=>y.
-  rewrite adj 2!gsup_spec 2!forall_image.
+  rewrite adj 2!gsup_spec 2!upper_bound_image.
   apply: forall_iff=>i.
-  by rewrite -adj. 
+  by rewrite -adj.
 Qed.
 
 (** ** standard supremum operations *)
@@ -336,7 +354,7 @@ HB.mixin Record PO_isup X of PO X := {
 HB.builders Context X of PO_isup X.
   Definition sup (P: X -> Prop) := isup P types_id.
   Lemma sup_spec (P: X -> Prop): is_sup P (sup P).
-  Proof. move: (isup_sup_spec P types_id). by rewrite image_id. Qed.
+  Proof. move: (isup_sup_spec P types_id)=>/=. by rewrite image_id'. Qed.
   HB.instance Definition _ := PO_cup.Build X _ (fun x y => sup_spec (pair x y)).
   HB.instance Definition _ := PO_dsup.Build X _ (fun D _ => sup_spec D).
 HB.end.
@@ -348,13 +366,13 @@ Arguments isup {_ _}.
 
 Notation sup P := (isup P types_id).
 Lemma sup_spec (X: supCL.type) (P: X -> Prop): is_sup P (sup P).
-Proof. move: (isup_sup_spec X P types_id). by rewrite image_id. Qed.
+Proof. move: (isup_sup_spec X P types_id). by rewrite image_id'. Qed.
 
 Section bot.
 Context {X: botPO.type}.
 Implicit Types x y z: X.  
 Lemma bot_spec z: bot <= z <-> True.
-Proof. by rewrite bot_sup_spec/=. Qed.
+Proof. by rewrite bot_sup_spec/upper_bound/=. Qed.
 Lemma geq_bot z: bot <= z.
 Proof. by rewrite bot_spec. Qed.
 Lemma leq_bot z: z <= bot -> z ≡ bot. (* iff, reversed? *)
@@ -371,7 +389,7 @@ Section cup.
 Context {X: joinSemiLattice.type}.
 Implicit Types x y z: X.  
 Lemma cup_spec x y z: cup x y <= z <-> x <= z /\ y <= z.
-Proof. by rewrite cup_sup_spec forall_pair. Qed.
+Proof. by rewrite cup_sup_spec upper_bound_pair. Qed.
 Lemma geq_cup x y z: x <= z -> y <= z -> cup x y <= z.
 Proof. move=>xz yz. by rewrite cup_spec. Qed.
 Lemma leq_cup_l x y z: z <= x -> z <= cup x y.
@@ -401,9 +419,8 @@ Qed.
 Lemma directed_sup_closure (P: X -> Prop): directed (sup_closure P).
 Proof.
   move=>x y Px Py. exists (cup x y). split.
-  apply: sc_sup. 2: exact: cup_sup_spec.
-  by setoid_rewrite forall_pair.
-  by apply cup_spec.
+  - apply: sc_sup. 2: exact: cup_sup_spec. by move=>t [<-|<-].
+  - exact/cup_spec.
 Qed.
 End cup.
 #[export] Hint Resolve leq_cup_l leq_cup_r: lattice.
@@ -437,7 +454,7 @@ End cpo.
 Lemma adj_csup {X Y: CPO.type} (f: X ⊣ Y) (P: X -> Prop) C: f (csup P C) ≡ csup (image f P) (chain_image f C). 
 Proof.
   apply: from_above=>y.
-  rewrite adj 2!csup_spec forall_image/=.
+  rewrite adj 2!csup_spec upper_bound_image.
   apply: forall_iff=>x.
   by rewrite -adj.
 Qed.
@@ -457,7 +474,7 @@ End dcpo.
 Lemma adj_dsup {X Y: dCPO.type} (f: X ⊣ Y) (P: X -> Prop) D: f (dsup P D) ≡ dsup (image f P) (directed_image f D). 
 Proof.
   apply: from_above=>y.
-  rewrite adj 2!dsup_spec forall_image/=.
+  rewrite adj 2!dsup_spec upper_bound_image.
   apply: forall_iff=>x.
   by rewrite -adj.
 Qed.
@@ -466,7 +483,7 @@ Section isup.
 Context {X: supCL.type}.
 Implicit Types x y z: X.  
 Lemma isup_spec I (P: I -> Prop) (h: I -> X) z: isup P h <= z <-> forall i, P i -> h i <= z.
-Proof. by rewrite isup_sup_spec forall_image. Qed.
+Proof. by rewrite isup_sup_spec upper_bound_image. Qed.
 Lemma geq_isup I (P: I -> Prop) (h: I -> X) (z: X): (forall i, P i -> h i <= z) -> isup P h <= z.
 Proof. move=>H. by rewrite isup_spec. Qed.
 Lemma leq_isup I (P: I -> Prop) (h: I -> X) i: P i -> h i <= isup P h.
@@ -559,7 +576,7 @@ End DIRECT_DPROD.
 Definition empty_kind: gkind := fun X _ => X -> False.
 Definition False_empty_kind: empty_kind False empty.
 Proof. done. Defined.
-Lemma image_empty_kind I P (H: empty_kind I P) X (f: I -> X): image f P ≡ empty.
+Lemma image_empty_kind I P (H: empty_kind I P) {X: Setoid.type} (f: I -> X): image f P ≡ empty.
 Proof. split=>//[[? _]]. exact: H. Qed. 
 
 Definition bot_gen (X: Type) := X.
@@ -597,15 +614,16 @@ HB.end.
 
 (** *** binary joins as generic sups over 2-element domains *)
 Record pair_kind (X: PO.type) (P: X -> Prop): Type :=
+  (* TOTHINK: use setoid pairs? *)
   indeed_pair { elem1; elem2; Pelem1: P elem1; Pelem2: P elem2;
                 all_there: forall z: X, z=elem1 \/ z=elem2 }.
 Definition bool_pair_kind: pair_kind (discrete bool) full.
 Proof. exists false true=>//. by case; auto. Defined.
-Lemma image_pair_kind I P (H: pair_kind I P) X (f: I -> X): image f P ≡ pair (f (elem1 H)) (f (elem2 H)).
+Lemma image_pair_kind I P (H: pair_kind I P) {X: Setoid.type} (f: I -> X): image f P ≡ pair (f (elem1 H)) (f (elem2 H)).
 Proof.
   split.
-  - move=>[i [Pi ->]]. rewrite /pair; case: (all_there H i)=>->; auto.
-  - move=>[->|->]; apply: in_image; apply H.
+  - move=>[i [Pi ->]]. rewrite /pair; case: (all_there H i)=>/=->; auto.
+  - case=>/=<-; apply: in_image; apply H.
 Qed.
 
 Definition cup_gen (X: Type) := X.
@@ -636,7 +654,7 @@ End s.
 
 Lemma cup_gsup_closed {X: joinSemiLattice.type} (P: X -> Prop) (Pcup: forall x y, P x -> P y -> P (cup x y)):
   @gsup_closed pair_kind (cup_gen X) P.
-Proof. move=>I Q kIQ h /forall_image H. apply: Pcup; apply: H; apply kIQ. Qed.
+Proof. move=>I Q kIQ h H. apply: Pcup; apply: H; apply kIQ. Qed.
 
 HB.factory Record comonadic_cup Y of PO Y := { X: joinSemiLattice.type; f: Y ⊢· X }.
 HB.builders Context Y of comonadic_cup Y.
@@ -653,7 +671,7 @@ Section s.
   Variables (P: X -> Prop) (D: chain P). 
   Definition gsup_csup := gsup X P D types_id.
   Lemma gsup_csup_spec: is_sup P gsup_csup.
-  Proof. move: (gsup_spec X P D types_id). by rewrite image_id. Qed.
+  Proof. move: (gsup_spec X P D types_id). by rewrite image_id'. Qed.
  End s.
  HB.instance Definition _ := PO_csup.Build (csup_gen X) _ gsup_csup_spec.
 End s.
@@ -668,9 +686,9 @@ Section s.
  HB.instance Definition _ := PO_gsup.Build (@chain) (csup_gen X) _ csup_gsup_spec. 
 End s.
 
-Lemma csup_gsup_closed {X: CPO.type} (P: X -> Prop) (Pcsup: forall Q (C: chain Q), Q <= P -> P (csup Q C)):
+Lemma csup_gsup_closed {X: CPO.type} (P: X -> Prop) (Pcsup: forall Q (C: chain Q), Q <= saturate P -> P (csup Q C)):
   @gsup_closed (@chain) (csup_gen X) P.
-Proof. move=>I Q kIQ h H. exact: Pcsup. Qed.
+Proof. move=>I Q kIQ h H. apply: Pcsup. exact/image_adj''. Qed.
 
 (** *** directed sups as generic sups over directed domains *)
 Definition dsup_gen (X: Type) := X.
@@ -681,7 +699,7 @@ Section s.
   Variables (P: X -> Prop) (D: directed P). 
   Definition gsup_dsup := gsup X P D types_id.
   Lemma gsup_dsup_spec: is_sup P gsup_dsup.
-  Proof. move: (gsup_spec X P D types_id). by rewrite image_id. Qed.
+  Proof. move: (gsup_spec X P D types_id). by rewrite image_id'. Qed.
  End s.
  HB.instance Definition _ := PO_dsup.Build (dsup_gen X) _ gsup_dsup_spec.
 End s.
@@ -696,9 +714,9 @@ Section s.
  HB.instance Definition _ := PO_gsup.Build (@directed) (dsup_gen X) _ dsup_gsup_spec. 
 End s.
 
-Lemma dsup_gsup_closed {X: dCPO.type} (P: X -> Prop) (Pdsup: forall Q (D: directed Q), Q <= P -> P (dsup Q D)):
+Lemma dsup_gsup_closed {X: dCPO.type} (P: X -> Prop) (Pdsup: forall Q (D: directed Q), Q <= saturate P -> P (dsup Q D)):
   @gsup_closed (@directed) (dsup_gen X) P.
-Proof. move=>I Q kIQ h H. exact: Pdsup. Qed.
+Proof. move=>I Q kIQ h H. apply: Pdsup. exact/image_adj''. Qed.
 
 (** *** indexed arbitrary sups as generic sups of arbitrary kind *)
 Definition any_kind: gkind := fun _ _ => True.
@@ -728,9 +746,9 @@ Section s.
  HB.instance Definition _ := PO_gsup.Build any_kind (isup_gen X) _ isup_gsup_spec. 
 End s.
 
-Lemma isup_gsup_closed {X: supCL.type} (P: X -> Prop) (Pisup: forall I (Q: I -> Prop) h, image h Q <= P -> P (isup Q h)):
+Lemma isup_gsup_closed {X: supCL.type} (P: X -> Prop) (Pisup: forall I (Q: I -> Prop) h, image h Q <= saturate P -> P (isup Q h)):
   @gsup_closed any_kind (isup_gen X) P.
-Proof. move=>I Q kIQ h H; exact: Pisup. Qed.
+Proof. move=>I Q kIQ h H; apply: Pisup. exact/image_adj''. Qed.
 
 (** liftings to dependent products [forall i, X i] follow generically *)
 (* HB.instance Definition _ I (X: I -> botPO.type) := botPO.copy (forall i, X i) (bot_gen (forall i, [gbot_for (X i)])). *)
@@ -756,13 +774,13 @@ HB.instance Definition _ (X: PO.type) (Y: supCL.type) := supCL.copy (X -mon-> Y)
 
 (** ** additional lemmas using suprema on subsets *)
 
-Lemma image_bot {X Y: Type} (f: X -> Y): image f bot ≡ bot.
+Lemma image_bot {X} {Y: Setoid.type} (f: X -> Y): image f bot ≡ bot.
 Proof. exact: image_empty. Qed.
-Lemma image_cup {X Y: Type} (f: X -> Y) (U V: X -> Prop): image f (cup U V) ≡ cup (image f U) (image f V).
+Lemma image_cup {X} {Y: Setoid.type} (f: X -> Y) (U V: X -> Prop): image f (cup U V) ≡ cup (image f U) (image f V).
 Proof. cbv. by firstorder. Qed.
-Lemma image_isup {X Y: Type} (f: X -> Y) I P (h: I -> X -> Prop): image f (isup P h) ≡ isup P (fun i => image f (h i)).
+Lemma image_isup {X} {Y: Setoid.type} (f: X -> Y) I P (h: I -> X -> Prop): image f (isup P h) ≡ isup P (fun i => image f (h i)).
 Proof. cbv. by firstorder. Qed.
-Lemma image_sup {X Y: Type} (f: X -> Y) (P: (X -> Prop) -> Prop): image f (sup P) ≡ isup P (image f).
+Lemma image_sup {X} {Y: Setoid.type} (f: X -> Y) (P: (X -> Prop) -> Prop): image f (sup P) ≡ isup P (image f).
 Proof. exact: image_isup. Qed.
 
 Lemma is_sup_cup {X: joinSemiLattice.type} U V (u v: X):
